\newpage
\section[Day 4: Euclidean Spaces \& Cauchy-Schwarz]
{Euclidean Spaces \& Cauchy-Schwarz}





\subsection{Euclidean Spaces}

	For each positive integer k, let $\mathbb{R}$$^\text{k}$ be the set of all ordered k-tuples:

	\qquad x = $(x_1,...,x_k)$	\qquad \qquad for each $x_i$ $\in$ $\mathbb{R}$

	with the properties:
	\begin{itemize}[leftmargin=1cm, itemsep=0.1cm]
		\item x+y = $(x_1+y_1,...,x_k+y_k)$ $\in$ $\mathbb{R}^{\text{k}}$
	
		\item cx = $(cx_1,...,cx_k)$ $\in$ $\mathbb{R}$$^\text{k}$
	\end{itemize}

	So, $\mathbb{R}$$^\text{n}$ has a vector space structure. Similarly, for $\mathbb{C}^{\text{n}}$. \\


{ \color{blue} Definition 4.1.1: Inner Product for $\mathbb{R}^k$}

	\begin{adjustbox}{minipage=14cm, right, vspace=0.1cm 0cm}
		$x \cdot y = x_1y_1 + ... + x_ky_k$ $\in$ $\mathbb{R}$ \\
	\end{adjustbox}

{ \color{blue} Definition 4.1.2: Norm }

	\begin{adjustbox}{minipage=14cm, right, vspace=0.1cm 0cm}
		$|x| = \sqrt{x \cdot x}$ = $\sqrt{\sum_{i=1}^k x_i^2}$ \\
	\end{adjustbox}

{ \color{blue} Definition 4.1.3: Extension to $\mathbb{C}^k$ } 

	\hspace{1cm}
	For z,w $\in$ $\mathbb{C}^n$
	
	\begin{itemize}[leftmargin=2cm, itemsep=0.1cm]
		\item $z \cdot w = z_1\overline{w_1} + ... + z_k\overline{w_k}$
	
		\item $z \cdot z = z_1\overline{z_1} + ... + z_k\overline{z_k}
			= |z_1|^2 + ... + |z_k|^2$ = $|z|^2$
	\end{itemize}





\subsection{Cauchy-Schwarz} 

{ \color{red} Theorem 4.2.1: Cauchy-Schwarz } 

	\begin{adjustbox}{minipage=14cm, right, vspace=0.1cm 0cm}
		If $\alpha_1 , ... , \alpha_n$ $\in$ $\mathbb{C}$ and
		$b_1 , ... , b_n$ $\in$ $\mathbb{C}$, then:

		\hspace{1cm}
		$| \sum_{\text{j=1}}^{n} a_j(\overline{b_j})  |^2 \leq
		\sum_{\text{j=1}}^{n} |a_j|^2 \sum_{\text{j=1}}^{n} |b_j|^2 $
	\end{adjustbox}

{ \color{magenta} \underline{Proof} }

	\fbox{
	\begin{minipage}{15cm}
		Let $A = \sum$ $|a_j|^2$ and $B = \sum$ $|b_j|^2$ and
		$C = \sum$ $a_j(\overline{b_j})$.

		If $B = 0$, then $b_1$ = ... = $b_n$ = 0. Thus, $0 \leq A(0)$ holds true.

		Suppose $B > 0$. Then:

		\hspace{1cm}
		$\sum$ $|Ba_j - Cb_j|^2$
		= $\sum$ $(Ba_j - Cb_j)\overline{(Ba_j - Cb_j)}$
		= $\sum$ $(Ba_j - Cb_j)(\overline{B} \ \overline{a_j}
		- \overline{C} \ \overline{b_j})$

		\hspace{1cm}
		= $\sum$ $(Ba_j-Cb_j)(B\overline{a_j} - \overline{C} \ \overline{b_j})$
		= $\sum$ $B^2a_j\overline{a_j} - B\overline{C}a_j\overline{b_j}
		- BC\overline{a_j}b_j + C\overline{C}b_j\overline{b_j}$

		\hspace{1cm}
		= $B^2 \sum |a_j|^2 - B\overline{C}\sum a_j\overline{b_j}
		- BC \sum \overline{a_j}b_j+ |C|^2 \sum |b_j|^2$

		\hspace{1cm}
		= $B^2A - B\overline{C}C - BC\overline{C} + |C|^2B$
		= $B^2A - 2|C|^2B + |C|^2B$ = $B^2A -|C|^2B$

		\hspace{1cm}
		= $B(AB - |C|^2)$

		Since $| Ba_j - Cb_j |$ $\geq$ 0, then $B(AB - |C|^2)$ $\geq$ 0.

		Since $B$ $>$ 0, then $AB - |C|^2$ $\geq$ 0 so $AB$ $\geq$ $|C|^2$.
	\end{minipage} }

	 \vspace{0.5cm}

{ \color{blue} Definition 4.2.2: Consequence of the Cauchy-Schwarz }

	\begin{adjustbox}{minipage=14cm, right, vspace=0.1cm 0cm}
		Since $|z_i|^2 = z_i\overline{z_i}$, then
		$\sum z_i\overline{z_i} = \sum |z_i|^2$ = $|z|^2$. Thus:

		\hspace{1cm}
		$|z \cdot w|^2$ = $|\sum z_i\overline{w_i} \ |^2$
		$\leq$ $\sum |z_i|^2 \sum |w_i|^2$ = $|z|^2$ $|w|^2$

		Thus, $|z \cdot w|$ $\leq$ $|z| |w|$.
	\end{adjustbox}

\newpage

{ \color{blue} Propositions 4.2.3 } 

	\hspace{1cm}
	Let $x,y,z$ $\in$ $\mathbb{R}^k$ where $\alpha$ $\in$ $\mathbb{R}$:
	
	\begin{enumerate}[label=(\alph*), leftmargin=2cm, itemsep=0.1cm]
		\item $|x|$ $\geq$ 0 where $|x| = 0$ only if x = 0

			{ \color{magenta} \underline{Proof} }

			\fbox{
			\begin{minipage}{13cm}
				$|x| = \sqrt{\sum_{i=1}^{k} x_i^2} \geq 0$ where $|x| = 0$
				only if $x_1 = ... = x_k = 0$ 
			\end{minipage} }

		\item $|\alpha x|$ = $|\alpha| |x|$

			{ \color{magenta} \underline{Proof} }

			\fbox{
			\begin{minipage}{13cm}
				$|\alpha x|$ = $\sqrt{\sum_{i=1}^k (\alpha x_i)^2}$
				= $\sqrt{\alpha^2} \sqrt{\sum_{i=1}^k x_i^2}$ = $|\alpha| |x|$
			\end{minipage} }
	
		\item $|x+y|$ $\leq$ $|x| + |y|$

			{ \color{magenta} \underline{Proof} }

			\fbox{
			\begin{minipage}{13cm}
				$|x+y|^2$ = $(x+y) \cdot (x+y)$ = $|x|^2 + 2(x \cdot y) + |y|^2$

				$\leq$ $|x|^2 + 2|x||y| + |y|^2$ = $(|x|+|y|)^2$
			\end{minipage} }

		\item $|x-y|$ $\leq$ $|x-z| + |y-z|$

			{ \color{magenta} \underline{Proof} }

			\fbox{
			\begin{minipage}{13cm}
				$|x-y|$ = $|x-z + z-y|$ $\leq$ $|x-z| + |z-y|$ = $|x-z| + |y-z|$
			\end{minipage} }
	\end{enumerate}

